Move the shared definitions between the compiler and templates to CodeGen.v/Correctess.v, and relax the definition of kernelInv with arbitrary resource

Compiler/Correctness.v
@@ -1,4 +1,4 @@
-Require Import Monad DepList GPUCSL TypedTerm Compiler.
+Require Import Monad DepList GPUCSL TypedTerm.
 Require Import Program.Equality LibTactics.
 Require Import CUDALib CSLLemma CodeGen CSLTactics.
 
@@ -43,14 +43,14 @@ Definition scInv {GS} (sVarEnv : SVarEnv GS) (sEvalEnv : SEvalEnv GS) :=
 
 Definition sexpInv {GS GA}
            (sVarEnv : SVarEnv GS) (sEvalEnv : SEvalEnv GS)
-           (aVarEnv : AVarEnv GA) (aPtrEnv : APtrEnv GA) (aEvalEnv : AEvalEnv GA) P resEnv :=
-  Assn (arrInvRes aPtrEnv aEvalEnv)
+           (aVarEnv : AVarEnv GA) (aPtrEnv : APtrEnv GA) (aEvalEnv : AEvalEnv GA) R P resEnv :=
+  Assn (arrInvRes aPtrEnv aEvalEnv *** R)
        P
        (resEnv ++ scInv sVarEnv sEvalEnv ++ arrInvVar aVarEnv aPtrEnv aEvalEnv).
 
 Definition kernelInv {GA} 
-           (aVarEnv : AVarEnv GA) (aPtrEnv : APtrEnv GA) (aEvalEnv : AEvalEnv GA) P resEnv := 
-  Assn (arrInvRes aPtrEnv aEvalEnv) P (resEnv ++ arrInvVar aVarEnv aPtrEnv aEvalEnv).
+           (aVarEnv : AVarEnv GA) (aPtrEnv : APtrEnv GA) (aEvalEnv : AEvalEnv GA) R P resEnv := 
+  Assn (arrInvRes aPtrEnv aEvalEnv *** R) P (resEnv ++ arrInvVar aVarEnv aPtrEnv aEvalEnv).
 
 Definition aenv_ok {GA} (avar_env : AVarEnv GA) :=
   (forall ty (m : member ty GA), prefix "l" (str_of_var (fst (hget avar_env m))) = false)
@@ -71,6 +71,12 @@ Definition is_local (x : var) : Prop := prefix "l" (str_of_var x) = true.
 Definition are_local {ty} (xs : vars ty) : Prop :=
   forall x, In x (flatTup xs) -> is_local x.
 
+Definition type_of_ftyp (fty : Skel.FTyp) :=
+  match fty with
+  | Skel.Fun1 dom cod => vars dom -> (cmd * vars cod)
+  | Skel.Fun2 dom1 dom2 cod => vars dom1 -> vars dom2 -> (cmd * vars cod)
+  end.
+
 Definition func_ok1 {GA dom cod} (avar_env : AVarEnv GA) 
            (f : Skel.Func GA (Skel.Fun1 dom cod)) (func : type_of_ftyp (Skel.Fun1 dom cod)) :=
   aenv_ok avar_env 
@@ -79,15 +85,15 @@ Definition func_ok1 {GA dom cod} (avar_env : AVarEnv GA)
      (* func only returs to local variables or parameter *)
      (forall x l, In l (flatTup (snd (func x))) -> is_local l) /\
      (* functional correctenss *)
-     (forall ntrd (tid : Fin.t ntrd) BS xs vs res aptr_env aeval_env P resEnv,
+     (forall ntrd (tid : Fin.t ntrd) BS xs vs res aptr_env aeval_env R P resEnv,
          (forall l, In l (flatTup xs) -> ~is_local l)
          -> (forall l v, In (l |-> v) resEnv -> ~is_local l)
          -> (Skel.funcDenote _ _ f aeval_env vs = Some res)
          -> CSL BS tid
-                (kernelInv avar_env aptr_env aeval_env P 
+                (kernelInv avar_env aptr_env aeval_env R P 
                            (xs |=> sc2CUDA vs ++ resEnv))
                 (fst (func xs))
-                (kernelInv avar_env aptr_env aeval_env P
+                (kernelInv avar_env aptr_env aeval_env R P
                            (snd (func xs) |=> sc2CUDA res ++
                             xs |=> sc2CUDA vs ++ resEnv))) /\
      (forall x, barriers (fst (func x)) = nil).
@@ -100,16 +106,16 @@ Definition func_ok2 {GA dom1 dom2 cod} (avar_env : AVarEnv GA)
      (* func only returs to local variables or parameter *)
      (forall x y l, In l (flatTup (snd (func x y))) -> is_local l) /\
      (* functional correctenss *)
-     (forall ntrd (tid : Fin.t ntrd) BS xs ys vs1 vs2 res aptr_env aeval_env P resEnv,
+     (forall ntrd (tid : Fin.t ntrd) BS xs ys vs1 vs2 res aptr_env aeval_env R P resEnv,
          (forall l, In l (flatTup xs) -> ~is_local l)
          -> (forall l, In l (flatTup ys) -> ~is_local l)
          -> (forall l v, In (l |-> v) resEnv -> ~is_local l)
          -> (Skel.funcDenote _ _ f aeval_env vs1 vs2 = Some res)
          -> CSL BS tid
-                (kernelInv avar_env aptr_env aeval_env P 
+                (kernelInv avar_env aptr_env aeval_env R P 
                            (xs |=> sc2CUDA vs1 ++ ys |=> sc2CUDA vs2 ++ resEnv))
                 (fst (func xs ys))
-                (kernelInv avar_env aptr_env aeval_env P
+                (kernelInv avar_env aptr_env aeval_env R P
                            (snd (func xs ys) |=> sc2CUDA res ++ 
                             xs |=> sc2CUDA vs1 ++ ys |=> sc2CUDA vs2 ++ resEnv))) /\
      (forall xs ys, barriers (fst (func xs ys)) = nil).
@@ -137,15 +143,15 @@ Definition ae_ok {GA ty} (avar_env : AVarEnv GA) (ae : Skel.AE GA ty) (arr : var
      (* func only returs to local variables or parameter *)
      (forall x l, In l (flatTup (snd (arr x))) -> is_local l) /\
      (* functional correctenss *)
-     (forall ntrd (tid : Fin.t ntrd) BS ix i res aptr_env aeval_env P resEnv,
+     (forall ntrd (tid : Fin.t ntrd) BS ix i res aptr_env aeval_env R P resEnv,
          ~is_local ix
          -> (forall l v, In (l |-> v) resEnv -> ~is_local l)
          -> (Skel.aeDenote _ _ ae aeval_env = Some res)
          -> i < length res
          -> CSL BS tid
-                (kernelInv avar_env aptr_env aeval_env P 
+                (kernelInv avar_env aptr_env aeval_env R P 
                            (ix |-> Zn i :: resEnv))
                 (fst (arr ix))
-                (kernelInv avar_env aptr_env aeval_env P
+                (kernelInv avar_env aptr_env aeval_env R P
                            ((snd (arr ix)) |=> sc2CUDA (gets' res i) ++ ix |-> Zn i :: resEnv))) /\
      (forall x, barriers (fst (arr x)) = nil).
